src/SepStep.v
@@ -1,0 +1,64 @@
+From Heapster Require Import
+     Permissions.
+
+From Coq Require Import
+     Classes.RelationClasses.
+
+Section step.
+
+  Context {config specConfig : Type}.
+
+  Definition sep_step (p q : @perm (config * specConfig)) : Prop :=
+    forall r, p ⊥ r -> q ⊥ r.
+
+  Global Instance sep_step_refl : Reflexive sep_step.
+  Proof.
+    repeat intro; auto.
+  Qed.
+
+  Global Instance sep_step_trans : Transitive sep_step.
+  Proof.
+    repeat intro. auto.
+  Qed.
+
+  Lemma sep_step_lte : forall p p' q, p <= p' -> sep_step p q -> sep_step p' q.
+  Proof.
+    repeat intro. apply H0. symmetry. symmetry in H1. eapply separate_antimonotone; eauto.
+  Qed.
+
+  Lemma sep_step_lte' : forall p q, q <= p -> sep_step p q.
+  Proof.
+    repeat intro. symmetry. eapply separate_antimonotone; eauto. symmetry; auto.
+  Qed.
+
+  Lemma sep_step_rely : forall p q x y, sep_step p q -> rely p x y -> rely q x y.
+  Proof.
+    intros. specialize (H (sym_guar_perm p) (separate_self_sym _)).
+    apply H; auto.
+  Qed.
+
+  Lemma sep_step_guar : forall p q x y, sep_step p q ->
+                                   guar q x y ->
+                                   guar p x y.
+  Proof.
+    intros. specialize (H (sym_guar_perm p) (separate_self_sym _)).
+    apply H; auto.
+  Qed.
+
+  Lemma sep_step_sep_conj_l : forall p1 p2 q, p1 ⊥ q -> sep_step p1 p2 -> sep_step (p1 ** q) (p2 ** q).
+  Proof.
+    intros p1 p2 q ? ?.
+    repeat intro; auto. symmetry in H1. symmetry. apply separate_sep_conj_perm; symmetry; auto.
+    - apply H0. symmetry. eapply separate_sep_conj_perm_l; eauto.
+    - symmetry. eapply separate_sep_conj_perm_r; eauto.
+  Qed.
+  Lemma sep_step_sep_conj_r : forall p1 p2 q, p1 ⊥ q -> sep_step p1 p2 -> sep_step (q ** p1) (q ** p2).
+  Proof.
+    intros p1 p2 q ? ?.
+    repeat intro; auto. symmetry in H1. symmetry. apply separate_sep_conj_perm; symmetry; auto.
+    - symmetry. eapply separate_sep_conj_perm_l; eauto.
+    - apply H0. symmetry. eapply separate_sep_conj_perm_r; eauto.
+    - symmetry. auto.
+  Qed.
+
+End step.
